theories/Congress_Buggy.v
@@ -202,8 +202,6 @@ Qed.
 
 End Equivalences.
 
-Definition version : Version := 1%nat.
-
 Definition validate_rules (rules : Rules) : bool :=
     (rules.(min_vote_count_permille) >=? 0)
         && (rules.(min_vote_count_permille) <=? 1000)
@@ -381,7 +379,7 @@ Lemma receive_proper :
 Proof. repeat intro; solve_contract_proper. Qed.
 
 Definition contract : Contract Setup Msg State :=
-  build_contract version init init_proper receive receive_proper.
+  build_contract init init_proper receive receive_proper.
 
 End CongressBuggy.
 (* We will show that this contract is buggy and does not satisfy the
@@ -421,7 +419,7 @@ Instance exploit_receive_proper :
 Proof. now subst. Qed.
 
 Definition exploit_contract : Contract ExploitSetup ExploitMsg ExploitState :=
-  build_contract 0 exploit_init exploit_init_proper exploit_receive exploit_receive_proper.
+  build_contract exploit_init exploit_init_proper exploit_receive exploit_receive_proper.
 
 End ExploitContract.
 
